src/StatDb/StatDbAPI.v
@@ -3,6 +3,9 @@ Require Import POCS.
 
 Definition State := list nat.
 
+Definition inited (s : State) : Prop :=
+  s = nil.
+
 Definition add_spec v : Specification unit unit unit State :=
   fun (_ : unit) state => {|
     pre := True;
@@ -31,10 +34,12 @@ Module Type StatDbAPI.
 
   Parameter abstr : Abstraction State.
 
+  Axiom init_ok : init_invariant init recover abstr inited.
   Axiom add_ok : forall v, prog_spec (add_spec v) (add v) recover abstr.
   Axiom mean_ok : prog_spec mean_spec mean recover abstr.
   Axiom recover_noop : rec_noop recover abstr no_crash.
 
+  Hint Resolve init_ok.
   Hint Resolve add_ok.
   Hint Resolve mean_ok.
   Hint Resolve recover_noop.
