src/Variables/VariablesImpl.v
@@ -4,31 +4,21 @@ Require Import VariablesAPI.
 
 Extraction Language Haskell.
 
-Axiom init : prog InitResult.
-Axiom read : var -> prog nat.
-Axiom write : var -> nat -> prog unit.
-Axiom recover : prog unit.
-
-Axiom abstr : Abstraction State.
-
-Axiom read_ok : forall v, prog_spec (read_spec v) (read v) recover abstr.
-Axiom write_ok : forall v val, prog_spec (write_spec v val) (write v val) recover abstr.
-Axiom recover_noop : rec_noop recover abstr no_crash.
-
 Module Vars <: VarsAPI.
 
-  Definition init := init.
-  Definition read := read.
-  Definition write := write.
-  Definition recover := recover.
+  Axiom init : prog InitResult.
+  Axiom read : var -> prog nat.
+  Axiom write : var -> nat -> prog unit.
+  Axiom recover : prog unit.
 
-  Definition abstr := abstr.
+  Axiom abstr : Abstraction State.
 
-  Definition read_ok := read_ok.
-  Definition write_ok := write_ok.
-  Definition recover_noop := recover_noop.
+  Axiom init_ok : init_invariant init recover abstr inited_any.
+  Axiom read_ok : forall v, prog_spec (read_spec v) (read v) recover abstr.
+  Axiom write_ok : forall v val, prog_spec (write_spec v val) (write v val) recover abstr.
+  Axiom recover_noop : rec_noop recover abstr no_crash.
 
 End Vars.
 
-Extract Constant read => "Variables.read".
-Extract Constant write => "Variables.write".
+Extract Constant Vars.read => "Variables.read".
+Extract Constant Vars.write => "Variables.write".
