src/StatDb/StatDbCli.v
@@ -3,7 +3,7 @@ Require Import StatDb.StatDbImpl.
 Require Import Variables.VariablesImpl.
 
 
-Module statdb := StatDB VariablesImpl.
+Module statdb := StatDB Vars.
 
 Axiom get_new_item : prog nat.
 Axiom report_mean : option nat -> prog unit.
